<?xml version="1.0"?>
<rdf:RDF xmlns="http://vocab.linkeddata.es/datosabiertos/def/common/zone#"
     xml:base="http://vocab.linkeddata.es/datosabiertos/def/common/zone"
     xmlns:dc="http://purl.org/dc/elements/1.1/"
     xmlns:owl="http://www.w3.org/2002/07/owl#"
     xmlns:rdf="http://www.w3.org/1999/02/22-rdf-syntax-ns#"
     xmlns:xml="http://www.w3.org/XML/1998/namespace"
     xmlns:xsd="http://www.w3.org/2001/XMLSchema#"
     xmlns:rdfs="http://www.w3.org/2000/01/rdf-schema#"
     xmlns:vann="http://purl.org/vocab/vann/"
     xmlns:terms="http://purl.org/dc/terms/">
    <owl:Ontology rdf:about="http://vocab.linkeddata.es/datosabiertos/def/common/zone#">
        <owl:imports rdf:resource="http://vocab.linkeddata.es/datosabiertos/def/sector-publico/territorio_v0.5"/>
        <owl:imports rdf:resource="http://vocab.linkeddata.es/datosabiertos/def/urbanismo-infraestructuras/callejero_v0.3"/>
        <dc:abstract xml:lang="es">Esta ontología tiene como propósito definir, categorizar y relacionar las Zonas Regulatorias en el contexto de la movilidad inteligente y la gestión urbana (Smart Cities). Se ha diseñado como una extensión modular de la ontología del Sector Público de España (esadm).</dc:abstract>
        <dc:abstract xml:lang="en">This ontology aims to define, categorize, and relate Regulatory Zones in the context of smart mobility and urban management (Smart Cities). It is designed as a modular extension of the Spanish Public Sector ontology (esadm).</dc:abstract>
        <dc:creator>OEG-UPM</dc:creator>
        <dc:title xml:lang="en">Base Zoning Ontology</dc:title>
        <dc:title xml:lang="es">Ontología base de Zonas</dc:title>
        <terms:issued rdf:datatype="http://www.w3.org/2001/XMLSchema#date">2026-01-27</terms:issued>
        <vann:preferredNamespacePrefix>edintzone</vann:preferredNamespacePrefix>
        <vann:preferredNamespaceUri>http://vocab.linkeddata.es/datosabiertos/def/common/zone#</vann:preferredNamespaceUri>
        <rdfs:comment xml:lang="es">Actualmente, existen vocabularios para divisiones administrativas (esadm) y geometrías (GeoSPARQL), pero existía un vacío semántico para representar entidades funcionales que se superponen a la trama urbana (ZBE, Carga y Descarga, etc...) sin responder a límites administrativos fijos. Esta ontología cubre dicho hueco.</rdfs:comment>
        <rdfs:comment xml:lang="en">Currently, vocabularies exist for administrative divisions (esadm) and geometries (GeoSPARQL), but there was a semantic gap for representing functional entities that overlay the urban grid (LEZ, Loading/Unloading, etc.) without adhering to fixed administrative boundaries. This ontology fills that gap.</rdfs:comment>
        <rdfs:label xml:lang="en">Base Zoning Ontology for Smart Mobility Use Case.</rdfs:label>
        <rdfs:label xml:lang="es">Ontología base de Zonas para el Caso de Uso de Movilidad Inteligente.</rdfs:label>
        <owl:versionInfo>0.1.0</owl:versionInfo>
    </owl:Ontology>
    


    <!-- 
    ///////////////////////////////////////////////////////////////////////////////////////
    //
    // Annotation properties
    //
    ///////////////////////////////////////////////////////////////////////////////////////
     -->


    


    <!-- http://purl.org/dc/elements/1.1/abstract -->


    <owl:AnnotationProperty rdf:about="http://purl.org/dc/elements/1.1/abstract"/>
    


    <!-- http://purl.org/dc/elements/1.1/creator -->


    <owl:AnnotationProperty rdf:about="http://purl.org/dc/elements/1.1/creator"/>
    


    <!-- http://purl.org/dc/elements/1.1/description -->


    <owl:AnnotationProperty rdf:about="http://purl.org/dc/elements/1.1/description"/>
    


    <!-- http://purl.org/dc/elements/1.1/title -->


    <owl:AnnotationProperty rdf:about="http://purl.org/dc/elements/1.1/title"/>
    


    <!-- http://purl.org/dc/terms/issued -->


    <owl:AnnotationProperty rdf:about="http://purl.org/dc/terms/issued"/>
    


    <!-- http://purl.org/vocab/vann/preferredNamespacePrefix -->


    <owl:AnnotationProperty rdf:about="http://purl.org/vocab/vann/preferredNamespacePrefix"/>
    


    <!-- http://purl.org/vocab/vann/preferredNamespaceUri -->


    <owl:AnnotationProperty rdf:about="http://purl.org/vocab/vann/preferredNamespaceUri"/>
    


    <!-- 
    ///////////////////////////////////////////////////////////////////////////////////////
    //
    // Datatypes
    //
    ///////////////////////////////////////////////////////////////////////////////////////
     -->


    


    <!-- http://www.opengis.net/ont/geosparql#wktLiteral -->


    <rdfs:Datatype rdf:about="http://www.opengis.net/ont/geosparql#wktLiteral"/>
    


    <!-- http://www.w3.org/2001/XMLSchema#date -->


    <rdfs:Datatype rdf:about="http://www.w3.org/2001/XMLSchema#date"/>
    


    <!-- 
    ///////////////////////////////////////////////////////////////////////////////////////
    //
    // Object Properties
    //
    ///////////////////////////////////////////////////////////////////////////////////////
     -->


    


    <!-- http://vocab.linkeddata.es/datosabiertos/def/common/zone#composedOf -->


    <owl:ObjectProperty rdf:about="http://vocab.linkeddata.es/datosabiertos/def/common/zone#composedOf">
        <rdfs:domain rdf:resource="http://vocab.linkeddata.es/datosabiertos/def/common/zone#RegulatedZone"/>
        <rdfs:range rdf:resource="http://dbpedia.org/ontology/GovernmentalAdministrativeRegion"/>
        <rdfs:range rdf:resource="http://www.geonames.org/ontology#Feature"/>
        <rdfs:comment xml:lang="es">Relación que permite definir una Zona Regulatoria mediante uno o más entidades administrativas (Via, Distrito, Municipio...).</rdfs:comment>
        <rdfs:comment xml:lang="en">Relationship that allows defining a Regulated Zone via one or more administrative entities (Street, District, Municipality...).</rdfs:comment>
        <rdfs:label xml:lang="en">composed of</rdfs:label>
        <rdfs:label xml:lang="es">compuesta por</rdfs:label>
    </owl:ObjectProperty>
    


    <!-- http://vocab.linkeddata.es/datosabiertos/def/common/zone#hasRegulatedZone -->


    <owl:ObjectProperty rdf:about="http://vocab.linkeddata.es/datosabiertos/def/common/zone#hasRegulatedZone">
        <owl:inverseOf rdf:resource="http://vocab.linkeddata.es/datosabiertos/def/common/zone#locatedIn"/>
        <rdfs:domain rdf:resource="http://vocab.linkeddata.es/datosabiertos/def/sector-publico/territorio#Municipio"/>
        <rdfs:range rdf:resource="http://vocab.linkeddata.es/datosabiertos/def/common/zone#RegulatedZone"/>
        <rdfs:comment xml:lang="en">Inverse property of &apos;locatedIn&apos;. Links a municipality with the regulated zones it contains.</rdfs:comment>
        <rdfs:comment xml:lang="es">Propiedad inversa de &apos;ubicado&apos;. Vincula un municipio con las zonas regulatorias que contiene.</rdfs:comment>
        <rdfs:label xml:lang="en">has regulated zone</rdfs:label>
        <rdfs:label xml:lang="es">tiene zona regulatoria</rdfs:label>
    </owl:ObjectProperty>
    


    <!-- http://vocab.linkeddata.es/datosabiertos/def/common/zone#locatedIn -->


    <owl:ObjectProperty rdf:about="http://vocab.linkeddata.es/datosabiertos/def/common/zone#locatedIn">
        <rdfs:subPropertyOf rdf:resource="http://www.opengis.net/ont/geosparql#sfWithin"/>
        <rdfs:domain rdf:resource="http://vocab.linkeddata.es/datosabiertos/def/common/zone#RegulatedZone"/>
        <rdfs:range rdf:resource="http://vocab.linkeddata.es/datosabiertos/def/sector-publico/territorio#Municipio"/>
        <rdfs:comment xml:lang="es">Relaciona una zona regulatoria con el municipio administrativo al que pertenece.</rdfs:comment>
        <rdfs:comment xml:lang="en">Relates a regulated zone to the administrative municipality it belongs to.</rdfs:comment>
        <rdfs:label xml:lang="en">located in municipality</rdfs:label>
        <rdfs:label xml:lang="es">ubicado en municipio</rdfs:label>
    </owl:ObjectProperty>
    


    <!-- http://vocab.linkeddata.es/datosabiertos/def/common/zone#managedBy -->


    <owl:ObjectProperty rdf:about="http://vocab.linkeddata.es/datosabiertos/def/common/zone#managedBy">
        <rdfs:domain rdf:resource="http://vocab.linkeddata.es/datosabiertos/def/common/zone#RegulatedZone"/>
        <rdfs:range rdf:resource="http://www.w3.org/ns/org#Organization"/>
        <rdfs:comment xml:lang="es">Organización (pública o privada) encargada de la gestión y operación de la zona.</rdfs:comment>
        <rdfs:comment xml:lang="en">Organization (public or private) responsible for the management and operation of the zone.</rdfs:comment>
        <rdfs:label xml:lang="es">entidad gestora</rdfs:label>
        <rdfs:label xml:lang="en">managed by</rdfs:label>
    </owl:ObjectProperty>
    


    <!-- http://www.opengis.net/ont/geosparql#hasGeometry -->


    <owl:ObjectProperty rdf:about="http://www.opengis.net/ont/geosparql#hasGeometry">
        <rdfs:label xml:lang="en">has geometry</rdfs:label>
        <rdfs:label xml:lang="es">tiene geometría</rdfs:label>
    </owl:ObjectProperty>
    


    <!-- http://www.opengis.net/ont/geosparql#sfWithin -->


    <owl:ObjectProperty rdf:about="http://www.opengis.net/ont/geosparql#sfWithin"/>
    


    <!-- 
    ///////////////////////////////////////////////////////////////////////////////////////
    //
    // Data properties
    //
    ///////////////////////////////////////////////////////////////////////////////////////
     -->


    


    <!-- http://vocab.linkeddata.es/datosabiertos/def/common/zone#endDate -->


    <owl:DatatypeProperty rdf:about="http://vocab.linkeddata.es/datosabiertos/def/common/zone#endDate">
        <rdfs:domain rdf:resource="http://vocab.linkeddata.es/datosabiertos/def/common/zone#RegulatedZone"/>
        <rdfs:range rdf:resource="http://www.w3.org/2001/XMLSchema#date"/>
        <rdfs:comment xml:lang="en">Date when the zone regulation ceases to be effective.</rdfs:comment>
        <rdfs:comment xml:lang="es">Fecha en la que la regulación de la zona deja de ser efectiva (derogación o fin de periodo).</rdfs:comment>
        <rdfs:label xml:lang="en">end date</rdfs:label>
        <rdfs:label xml:lang="es">fecha de fin de vigor</rdfs:label>
    </owl:DatatypeProperty>
    


    <!-- http://vocab.linkeddata.es/datosabiertos/def/common/zone#legalReference -->


    <owl:DatatypeProperty rdf:about="http://vocab.linkeddata.es/datosabiertos/def/common/zone#legalReference">
        <rdfs:domain rdf:resource="http://vocab.linkeddata.es/datosabiertos/def/common/zone#RegulatedZone"/>
        <rdfs:range rdf:resource="http://www.w3.org/2001/XMLSchema#anyURI"/>
        <rdfs:comment xml:lang="es">Enlace al documento oficial (Boletín, Ordenanza) que establece la creación de la zona.</rdfs:comment>
        <rdfs:comment xml:lang="en">Link to the official document (Bulletin, Ordinance) establishing the zone.</rdfs:comment>
        <rdfs:label xml:lang="en">legal reference</rdfs:label>
        <rdfs:label xml:lang="es">referencia legal</rdfs:label>
    </owl:DatatypeProperty>
    


    <!-- http://vocab.linkeddata.es/datosabiertos/def/common/zone#scheduleDescription -->


    <owl:DatatypeProperty rdf:about="http://vocab.linkeddata.es/datosabiertos/def/common/zone#scheduleDescription">
        <rdfs:domain rdf:resource="http://vocab.linkeddata.es/datosabiertos/def/common/zone#RegulatedZone"/>
        <rdfs:range rdf:resource="http://www.w3.org/2001/XMLSchema#string"/>
        <rdfs:comment xml:lang="es">Descripción textual del horario de funcionamiento de la zona (ej. &quot;Lunes a Viernes de 07:00 a 20:00&quot;).</rdfs:comment>
        <rdfs:comment xml:lang="en">Textual description of the zone&apos;s operating schedule (e.g., &quot;Monday to Friday from 07:00 to 20:00&quot;).</rdfs:comment>
        <rdfs:label xml:lang="es">horario descriptivo</rdfs:label>
        <rdfs:label xml:lang="en">schedule description</rdfs:label>
    </owl:DatatypeProperty>
    


    <!-- http://vocab.linkeddata.es/datosabiertos/def/common/zone#startDate -->


    <owl:DatatypeProperty rdf:about="http://vocab.linkeddata.es/datosabiertos/def/common/zone#startDate">
        <rdfs:domain rdf:resource="http://vocab.linkeddata.es/datosabiertos/def/common/zone#RegulatedZone"/>
        <rdfs:range rdf:resource="http://www.w3.org/2001/XMLSchema#date"/>
        <rdfs:comment xml:lang="en">Date from which the zone regulation becomes effective.</rdfs:comment>
        <rdfs:comment xml:lang="es">Fecha a partir de la cual la regulación de la zona comienza a ser efectiva.</rdfs:comment>
        <rdfs:label xml:lang="en">entry into force date</rdfs:label>
        <rdfs:label xml:lang="es">fecha de entrada en vigor</rdfs:label>
    </owl:DatatypeProperty>
    


    <!-- http://www.opengis.net/ont/geosparql#asWKT -->


    <owl:DatatypeProperty rdf:about="http://www.opengis.net/ont/geosparql#asWKT">
        <rdfs:domain rdf:resource="http://www.opengis.net/ont/sf#Geometry"/>
        <rdfs:range rdf:resource="http://www.opengis.net/ont/geosparql#wktLiteral"/>
        <rdfs:comment xml:lang="en">Geometry representation in Well-Known Text format.</rdfs:comment>
        <rdfs:comment xml:lang="es">Representación de la geometría en formato Well-Known Text.</rdfs:comment>
        <rdfs:label xml:lang="en">as WKT</rdfs:label>
        <rdfs:label xml:lang="es">como WKT</rdfs:label>
    </owl:DatatypeProperty>
    


    <!-- 
    ///////////////////////////////////////////////////////////////////////////////////////
    //
    // Classes
    //
    ///////////////////////////////////////////////////////////////////////////////////////
     -->


    


    <!-- http://dbpedia.org/ontology/GovernmentalAdministrativeRegion -->


    <owl:Class rdf:about="http://dbpedia.org/ontology/GovernmentalAdministrativeRegion"/>
    


    <!-- http://vocab.linkeddata.es/datosabiertos/def/common/zone#EconomicInterestZone -->


    <owl:Class rdf:about="http://vocab.linkeddata.es/datosabiertos/def/common/zone#EconomicInterestZone">
        <rdfs:subClassOf rdf:resource="http://vocab.linkeddata.es/datosabiertos/def/common/zone#RegulatedZone"/>
        <rdfs:comment xml:lang="en">Area delimited by municipal regulations to promote commercial or tourist activities.</rdfs:comment>
        <rdfs:comment xml:lang="es">Área delimitada por normativas municipales para fomentar actividades comerciales o turísticas.</rdfs:comment>
        <rdfs:label xml:lang="en">Economic Interest Zone</rdfs:label>
        <rdfs:label xml:lang="es">Zona de Interés Económico</rdfs:label>
    </owl:Class>
    


    <!-- http://vocab.linkeddata.es/datosabiertos/def/common/zone#FreeTradeZone -->


    <owl:Class rdf:about="http://vocab.linkeddata.es/datosabiertos/def/common/zone#FreeTradeZone">
        <rdfs:subClassOf rdf:resource="http://vocab.linkeddata.es/datosabiertos/def/common/zone#EconomicInterestZone"/>
        <rdfs:comment xml:lang="en">Area of the Union customs territory where non-Community goods are considered not situated within customs territory.</rdfs:comment>
        <rdfs:comment xml:lang="es">Área del territorio aduanero de la Unión donde las mercancías no comunitarias se consideran no situadas en territorio aduanero.</rdfs:comment>
        <rdfs:label xml:lang="en">Free Trade Zone</rdfs:label>
        <rdfs:label xml:lang="es">Zona Franca</rdfs:label>
    </owl:Class>
    


    <!-- http://vocab.linkeddata.es/datosabiertos/def/common/zone#HighTourismInfluxZone -->


    <owl:Class rdf:about="http://vocab.linkeddata.es/datosabiertos/def/common/zone#HighTourismInfluxZone">
        <rdfs:subClassOf rdf:resource="http://vocab.linkeddata.es/datosabiertos/def/common/zone#EconomicInterestZone"/>
        <rdfs:comment xml:lang="es">Zonas con gran afluencia turística donde se aplica plena libertad de apertura comercial en domingos y festivos.</rdfs:comment>
        <rdfs:comment xml:lang="en">Zones with high tourist influx where full freedom of commercial opening on Sundays and holidays applies.</rdfs:comment>
        <rdfs:label xml:lang="en">High Tourism Influx Zone</rdfs:label>
        <rdfs:label xml:lang="es">Zona de Gran Afluencia Turística</rdfs:label>
    </owl:Class>
    


    <!-- http://vocab.linkeddata.es/datosabiertos/def/common/zone#HistoricalCenter -->


    <owl:Class rdf:about="http://vocab.linkeddata.es/datosabiertos/def/common/zone#HistoricalCenter">
        <rdfs:subClassOf rdf:resource="http://vocab.linkeddata.es/datosabiertos/def/common/zone#RegulatedZone"/>
        <rdfs:comment xml:lang="en">Urban area with special heritage protection where strict restrictions on access, circulation, and parking apply to preserve the historical fabric.</rdfs:comment>
        <rdfs:comment xml:lang="es">Área urbana de especial protección patrimonial donde se aplican restricciones estrictas de acceso, circulación y estacionamiento para preservar la trama histórica.</rdfs:comment>
        <rdfs:label xml:lang="es">Casco Histórico</rdfs:label>
        <rdfs:label xml:lang="en">Historical Center</rdfs:label>
    </owl:Class>
    


    <!-- http://vocab.linkeddata.es/datosabiertos/def/common/zone#LoadingUnloadingZone -->


    <owl:Class rdf:about="http://vocab.linkeddata.es/datosabiertos/def/common/zone#LoadingUnloadingZone">
        <rdfs:subClassOf rdf:resource="http://vocab.linkeddata.es/datosabiertos/def/common/zone#RegulatedParkingZone"/>
        <rdfs:comment xml:lang="es">Zona reservada exclusivamente para la parada técnica de vehículos profesionales dedicados a la Distribución Urbana de Mercancías (DUM).</rdfs:comment>
        <rdfs:comment xml:lang="en">Zone reserved exclusively for the technical stop of professional vehicles dedicated to Urban Goods Distribution.</rdfs:comment>
        <rdfs:label xml:lang="en">Loading and Unloading Zone</rdfs:label>
        <rdfs:label xml:lang="es">Zona de Carga y Descarga</rdfs:label>
    </owl:Class>
    


    <!-- http://vocab.linkeddata.es/datosabiertos/def/common/zone#LogisticsActivityZone -->


    <owl:Class rdf:about="http://vocab.linkeddata.es/datosabiertos/def/common/zone#LogisticsActivityZone">
        <rdfs:subClassOf rdf:resource="http://vocab.linkeddata.es/datosabiertos/def/common/zone#EconomicInterestZone"/>
        <rdfs:comment xml:lang="es">Infraestructura especializada en actividades de transporte y logística. Definida legalmente como &apos;Centro de Transporte y Logística&apos;.</rdfs:comment>
        <rdfs:comment xml:lang="en">Infrastructure specialized in transport and logistics activities. Legally defined as &apos;Transport and Logistics Center&apos;.</rdfs:comment>
        <rdfs:label xml:lang="en">Logistics Activity Zone</rdfs:label>
        <rdfs:label xml:lang="es">Zona de Actividad Logística</rdfs:label>
    </owl:Class>
    


    <!-- http://vocab.linkeddata.es/datosabiertos/def/common/zone#LowEmissionZone -->


    <owl:Class rdf:about="http://vocab.linkeddata.es/datosabiertos/def/common/zone#LowEmissionZone">
        <rdfs:subClassOf rdf:resource="http://vocab.linkeddata.es/datosabiertos/def/common/zone#RegulatedZone"/>
        <rdfs:comment xml:lang="es">Zona definida por la administración donde se aplican restricciones de acceso, circulación y estacionamiento de vehículos con el objetivo de mejorar la calidad del aire.</rdfs:comment>
        <rdfs:comment xml:lang="en">Zone defined by the administration where restrictions on vehicle access, circulation, and parking apply to improve air quality.</rdfs:comment>
        <rdfs:label xml:lang="en">Low Emission Zone</rdfs:label>
        <rdfs:label xml:lang="es">Zona de Bajas Emisiones</rdfs:label>
    </owl:Class>
    


    <!-- http://vocab.linkeddata.es/datosabiertos/def/common/zone#ParkAndRideZone -->


    <owl:Class rdf:about="http://vocab.linkeddata.es/datosabiertos/def/common/zone#ParkAndRideZone">
        <rdfs:subClassOf rdf:resource="http://vocab.linkeddata.es/datosabiertos/def/common/zone#RegulatedParkingZone"/>
        <rdfs:comment xml:lang="en">Strategic parking zone located on the periphery and connected to public transport networks.</rdfs:comment>
        <rdfs:comment xml:lang="es">Zona de estacionamiento estratégico situado en la periferia y conectado con redes de transporte público.</rdfs:comment>
        <rdfs:label xml:lang="en">Park and Ride Zone</rdfs:label>
        <rdfs:label xml:lang="es">Zona de Estacionamiento Disuasorio</rdfs:label>
    </owl:Class>
    


    <!-- http://vocab.linkeddata.es/datosabiertos/def/common/zone#RegulatedParkingZone -->


    <owl:Class rdf:about="http://vocab.linkeddata.es/datosabiertos/def/common/zone#RegulatedParkingZone">
        <rdfs:subClassOf rdf:resource="http://vocab.linkeddata.es/datosabiertos/def/common/zone#RegulatedZone"/>
        <rdfs:comment xml:lang="en">Public road zone where parking is subject to time regulation, fee payment, or other restrictions.</rdfs:comment>
        <rdfs:comment xml:lang="es">Zona de la vía pública donde el estacionamiento está sujeto a regulación horaria, pago de tasas u otras restricciones.</rdfs:comment>
        <rdfs:label xml:lang="en">Regulated Parking Zone</rdfs:label>
        <rdfs:label xml:lang="es">Zona de Estacionamiento Regulado</rdfs:label>
    </owl:Class>
    


    <!-- http://vocab.linkeddata.es/datosabiertos/def/common/zone#RegulatedZone -->


    <owl:Class rdf:about="http://vocab.linkeddata.es/datosabiertos/def/common/zone#RegulatedZone">
        <rdfs:subClassOf rdf:resource="http://www.opengis.net/ont/geosparql#Feature"/>
        <rdfs:subClassOf>
            <owl:Restriction>
                <owl:onProperty rdf:resource="http://www.opengis.net/ont/geosparql#hasGeometry"/>
                <owl:someValuesFrom rdf:resource="http://www.opengis.net/ont/sf#Geometry"/>
            </owl:Restriction>
        </rdfs:subClassOf>
        <rdfs:subClassOf>
            <owl:Restriction>
                <owl:onProperty rdf:resource="http://vocab.linkeddata.es/datosabiertos/def/common/zone#locatedIn"/>
                <owl:qualifiedCardinality rdf:datatype="http://www.w3.org/2001/XMLSchema#nonNegativeInteger">1</owl:qualifiedCardinality>
                <owl:onClass rdf:resource="http://vocab.linkeddata.es/datosabiertos/def/sector-publico/territorio#Municipio"/>
            </owl:Restriction>
        </rdfs:subClassOf>
        <rdfs:comment xml:lang="es">Area a la que se aplica una regulacion o normativa particular</rdfs:comment>
        <rdfs:comment xml:lang="en">Area to which a particular regulation or policy applies</rdfs:comment>
        <rdfs:label xml:lang="en">Regulated Zone</rdfs:label>
        <rdfs:label xml:lang="es">Zona regulatoria</rdfs:label>
    </owl:Class>
    


    <!-- http://vocab.linkeddata.es/datosabiertos/def/common/zone#RegulatorySandbox -->


    <owl:Class rdf:about="http://vocab.linkeddata.es/datosabiertos/def/common/zone#RegulatorySandbox">
        <rdfs:subClassOf rdf:resource="http://vocab.linkeddata.es/datosabiertos/def/common/zone#EconomicInterestZone"/>
        <rdfs:comment xml:lang="en">Controlled testing environment authorized for research trials with automated vehicles or new forms of mobility.</rdfs:comment>
        <rdfs:comment xml:lang="es">Espacio controlado de pruebas autorizado para la realización de ensayos de investigación con vehículos automatizados o nuevas formas de movilidad.</rdfs:comment>
        <rdfs:label xml:lang="en">Regulatory Sandbox</rdfs:label>
        <rdfs:label xml:lang="es">Sandbox Regulatorio</rdfs:label>
    </owl:Class>
    


    <!-- http://vocab.linkeddata.es/datosabiertos/def/common/zone#ResidentialParkingZone -->


    <owl:Class rdf:about="http://vocab.linkeddata.es/datosabiertos/def/common/zone#ResidentialParkingZone">
        <rdfs:subClassOf rdf:resource="http://vocab.linkeddata.es/datosabiertos/def/common/zone#RegulatedParkingZone"/>
        <rdfs:comment xml:lang="es">Zona destinada prioritaria o exclusivamente al estacionamiento de vehículos de residentes empadronados.</rdfs:comment>
        <rdfs:comment xml:lang="en">Zone intended primarily or exclusively for parking vehicles of registered residents.</rdfs:comment>
        <rdfs:label xml:lang="en">Residential Parking Zone</rdfs:label>
        <rdfs:label xml:lang="es">Zona de Estacionamiento Residencial</rdfs:label>
    </owl:Class>
    


    <!-- http://vocab.linkeddata.es/datosabiertos/def/common/zone#ScienceTechnologyPark -->


    <owl:Class rdf:about="http://vocab.linkeddata.es/datosabiertos/def/common/zone#ScienceTechnologyPark">
        <rdfs:subClassOf rdf:resource="http://vocab.linkeddata.es/datosabiertos/def/common/zone#EconomicInterestZone"/>
        <rdfs:comment xml:lang="es">Espacio físico para el fomento de la I+D+i y la transferencia de conocimiento.</rdfs:comment>
        <rdfs:comment xml:lang="en">Physical space for promoting R&amp;D&amp;I and knowledge transfer.</rdfs:comment>
        <rdfs:label xml:lang="es">Parque Científico y Tecnológico</rdfs:label>
        <rdfs:label xml:lang="en">Science and Technology Park</rdfs:label>
    </owl:Class>
    


    <!-- http://vocab.linkeddata.es/datosabiertos/def/common/zone#ShortTermParkingZone -->


    <owl:Class rdf:about="http://vocab.linkeddata.es/datosabiertos/def/common/zone#ShortTermParkingZone">
        <rdfs:subClassOf rdf:resource="http://vocab.linkeddata.es/datosabiertos/def/common/zone#RegulatedParkingZone"/>
        <rdfs:comment xml:lang="es">Zona destinada principalmente a usuarios visitantes con limitación temporal estricta y tarificación para favorecer la alta rotación.</rdfs:comment>
        <rdfs:comment xml:lang="en">Zone intended primarily for visitors with strict time limits and fees to encourage high vehicle turnover.</rdfs:comment>
        <rdfs:label xml:lang="en">Short-term Parking Zone</rdfs:label>
        <rdfs:label xml:lang="es">Zona de Estacionamiento de Rotación</rdfs:label>
    </owl:Class>
    


    <!-- http://vocab.linkeddata.es/datosabiertos/def/common/zone#StreetVendingZone -->


    <owl:Class rdf:about="http://vocab.linkeddata.es/datosabiertos/def/common/zone#StreetVendingZone">
        <rdfs:subClassOf rdf:resource="http://vocab.linkeddata.es/datosabiertos/def/common/zone#EconomicInterestZone"/>
        <rdfs:comment xml:lang="es">Zona acotada para la modalidad de venta realizada fuera de establecimiento comercial permanente (mercadillos).</rdfs:comment>
        <rdfs:comment xml:lang="en">Zone demarcated for sales conducted outside of permanent commercial establishments (street markets).</rdfs:comment>
        <rdfs:label xml:lang="en">Street Vending Zone</rdfs:label>
        <rdfs:label xml:lang="es">Zona de Venta Ambulante</rdfs:label>
    </owl:Class>
    


    <!-- http://vocab.linkeddata.es/datosabiertos/def/sector-publico/territorio#Municipio -->


    <owl:Class rdf:about="http://vocab.linkeddata.es/datosabiertos/def/sector-publico/territorio#Municipio"/>
    


    <!-- http://www.geonames.org/ontology#Feature -->


    <owl:Class rdf:about="http://www.geonames.org/ontology#Feature"/>
    


    <!-- http://www.opengis.net/ont/geosparql#Feature -->


    <owl:Class rdf:about="http://www.opengis.net/ont/geosparql#Feature"/>
    


    <!-- http://www.opengis.net/ont/sf#Geometry -->


    <owl:Class rdf:about="http://www.opengis.net/ont/sf#Geometry"/>
    


    <!-- http://www.w3.org/ns/org#Organization -->


    <owl:Class rdf:about="http://www.w3.org/ns/org#Organization"/>
</rdf:RDF>



<!-- Generated by the OWL API (version 5.1.18) https://github.com/owlcs/owlapi/ -->


